theories/Math/OrderTheory.v
@@ -20,3 +20,17 @@ Qed.
 Next Obligation.
   intros x y. cbn. unfold flip. split; firstorder try congruence. contradiction (StrictOrder_Irreflexive x). firstorder.
 Qed.
+
+Class isWellOrderedSet (A : Type) : Type :=
+  { wltProp (lhs : A) (rhs : A) : Prop
+  ; wltProp_Transitive :: Transitive wltProp
+  ; wltProp_well_founded : well_founded wltProp
+  }.
+
+Infix "⪵" := wltProp : type_scope.
+
+#[global]
+Instance wltProp_StrictOrder {A : Type} `{WOSET : isWellOrderedSet A} : StrictOrder wltProp :=
+  { StrictOrder_Irreflexive := well_founded_implies_Irreflexive wltProp wltProp_well_founded
+  ; StrictOrder_Transitive := wltProp_Transitive
+  }.
