theories/Prelude/Notations.v
@@ -4,12 +4,14 @@ Reserved Infix "==" (no associativity, at level 70).
 Reserved Infix "=<" (no associativity, at level 70).
 Reserved Infix "≦" (at level 70, no associativity).
 
-Reserved Infix "\in" (no associativity, at level 70).
-Reserved Infix "\subseteq" (no associativity, at level 70).
-
 Reserved Infix "≦ᵣ" (at level 70, no associativity).
 Reserved Infix "=ᵣ" (at level 70, no associativity).
 Reserved Infix "<ᵣ" (at level 70, no associativity).
+
+Reserved Infix "⪵" (at level 70, no associativity).
+
+Reserved Infix "\in" (no associativity, at level 70).
+Reserved Infix "\subseteq" (no associativity, at level 70).
 
 Reserved Infix "$" (at level 100, right associativity).
 Reserved Infix ">>=" (at level 90, left associativity).
